SN without diamond in LF (sub)lang finished

Normalization/LF_NoDiamond.v
@@ -259,32 +259,37 @@ match M with
 | unbox_LF M => unbox_LF (SL L M)
 end.
 
-Lemma SL_lam:
-forall L M A,
-  SL L (lam_LF A M) = lam_LF A (SL L M).
-induction L; intros; simpl in *; auto; destruct a; destruct p;
-rewrite IHL; auto.
+Lemma Mem_concat_mem_elem:
+forall G (e:var*ty),
+  Mem e (concat G) ->
+  exists (l: ctx_LF), Mem l G /\ Mem e l.
+induction G; intros; rew_concat in *.
+rewrite Mem_nil_eq in H; contradiction.
+rewrite Mem_app_or_eq in H; destruct H.
+exists a; split; auto; apply Mem_here.
+destruct (IHG e); auto; destruct H0; exists x; split; auto.
+rewrite Mem_cons_eq; right; auto.
 Qed.
 
-Lemma SL_appl:
-forall L M N,
-  SL L (appl_LF M N) = appl_LF (SL L M) (SL L N).
-induction L; intros; simpl in *; auto; destruct a; destruct p;
-rewrite IHL; auto.
-Qed.
-
-Lemma SL_box:
-forall L M,
-  SL L (box_LF M) = box_LF (SL L M).
-induction L; intros; simpl in *; auto; destruct a; destruct p;
-rewrite IHL; auto.
-Qed.
-
-Lemma SL_unbox:
-forall L M,
-  SL L (unbox_LF M) = unbox_LF (SL L M).
-induction L; intros; simpl in *; auto; destruct a; destruct p;
-rewrite IHL; auto.
+Lemma ok_LF_Mem_Mem_eq':
+  forall (G : ctx_LF)(v : var) (A B : ty),
+    ok_LF G nil  ->
+    Mem (v, A) G -> Mem (v,B) G ->
+    A = B.
+induction G; intros.
+rewrite Mem_nil_eq in H0; contradiction.
+rewrite Mem_cons_eq in *; destruct H0; destruct H1; subst.
+inversion H1; subst; auto.
+inversion H; subst; apply Mem_split in H1; destruct H1 as (hd, (tl, H1));
+assert (hd & (v, B) ++ tl *=* (v, B) :: hd ++ tl) by permut_simpl;
+rewrite H1 in H6; apply ok_LF_permut with (G':= (v, B) :: hd ++ tl) in H6;
+auto; inversion H6; subst; elim H8; apply Mem_here.
+inversion H; subst; apply Mem_split in H0; destruct H0 as (hd, (tl, H0));
+assert (hd & (v, A) ++ tl *=* (v, A) :: hd ++ tl) by permut_simpl;
+rewrite H0 in H6; apply ok_LF_permut with (G':= (v, A) :: hd ++ tl) in H6;
+auto; inversion H6; subst; elim H8; apply Mem_here.
+eapply IHG; eauto.
+inversion H; subst; eapply ok_LF_used_weakening; eauto.
 Qed.
 
 Lemma SL_hyp:
@@ -300,33 +305,180 @@ inversion H1; subst; rewrite Mem_nil_eq in *; contradiction.
 destruct a; destruct p; inversion H1; subst; simpl in *.
 case_if.
 assert (A = t0).
-  (* from H and H5 *) skip.
+unfold ok_Bg_LF in *.
+apply ok_LF_Mem_Mem_eq' with (concat (Gamma::G)) v0; auto;
+[rew_concat; rewrite Mem_app_or_eq; left; auto | ].
+apply Mem_permut with (l:=(v0,t0) :: map fst_ L); [symmetry; auto |
+apply Mem_here].
 subst; apply H0 with v0; apply Mem_here.
 assert (concat (Gamma :: G) *=* (v0, t0) :: map fst_ L) by auto;
 symmetry in H; apply permut_split_head in H;
 destruct H as (hd, (tl, H)).
-assert (exists Gamma' G', concat (Gamma :: G) *=*
-                                 (v0,t0) :: concat (Gamma' :: G')).
-skip.
-destruct H4 as (Gamma', (G', H4)).
-apply IHL with G' Gamma'.
+destruct Mem_concat_mem_elem with (e:=(v0, t0)) (G:=Gamma::G).
+apply Mem_permut with (l:=(v0,t0) :: map fst_ L); [symmetry; auto |];
+apply Mem_here. destruct H4.
+apply Mem_split in H4.
+apply Mem_split in H6.
+destruct H6 as (l0, (l1,H6)).
+destruct H4 as (G0, (G1, H4)); subst.
+destruct G0; rew_app in *.
+inversion H4; subst. apply IHL with G1 (l0++l1).
+rew_concat in *.
 apply permut_cons_inv with (a:=(v0,t0)).
-rewrite <- H4. rewrite H3; auto.
-intros. apply H0 with a; rewrite Mem_cons_eq; right; auto.
-skip (* v <> v0 + H5 *).
+rewrite <- H3. permut_simpl.
+intros; apply H0 with a; rewrite Mem_cons_eq; right; auto.
+constructor.
+eapply ok_Bg_LF_permut_first_tail in Ok; eauto; permut_simpl.
+rewrite Mem_app_or_eq in *; destruct H5; auto; rewrite Mem_cons_eq in *;
+destruct H5; auto; inversion H5; subst; elim H2; auto.
+inversion H4; subst.
+apply IHL with (G0 ++ (l0 ++ l1) :: G1) c.
+rew_concat in *. apply permut_cons_inv with (a:=(v0,t0)).
+rewrite <- H3. permut_simpl.
+intros; apply H0 with a; rewrite Mem_cons_eq; right; auto.
+constructor; auto.
+assert (c :: G0 ++ (l0 ++ (v0, t0) :: l1) :: G1 ~=~
+        ((l0++(v0, t0) :: l1) :: c :: G0 ++ G1)).
+PPermut_LF_simpl; constructor; auto; permut_simpl.
+rewrite H6 in Ok.
+eapply ok_Bg_LF_permut_first_tail with (x:=v0)(A:=t0) (C':=l0++l1)in Ok; eauto.
+Focus 2. permut_simpl.
+apply ok_Bg_LF_PPermut with (G:=(l0 ++ l1) :: c :: G0 ++ G1); auto;
+PPermut_LF_simpl.
+Qed.
+
+Lemma closed_t_succ:
+forall M n,
+  lc_t_n_LF n M -> lc_t_n_LF (S n) M.
+intros; generalize dependent n;
+induction M; intros; inversion H; subst;
+eauto using lc_t_n_LF.
+Qed.
+
+Lemma closed_t_addition:
+forall M n m,
+  lc_t_n_LF n M -> lc_t_n_LF (n + m) M.
+intros; induction m;
+[ replace (n+0) with n by auto |
+  replace (n + S m) with (S (n+m)) by auto] ;
+try apply closed_t_succ;
+assumption.
+Qed.
+
+Lemma SL_nil:
+forall M,
+  SL nil M = M.
+induction M; intros; simpl in *;
+try erewrite IHM || (erewrite IHM1; erewrite IHM2); eauto.
+destruct v; auto.
+Qed.
+
+Lemma Mem_find_var:
+  forall L v,
+    Mem v (map fst_ (map fst_ L)) ->
+    exists A M, find_var L v = Some (v, A, M).
+induction L; intros; [ rewrite Mem_nil_eq in *; contradiction | ];
+destruct a; destruct p; rew_map in *; simpl in *.
+subst; rewrite Mem_cons_eq in H.
+destruct (eq_var_dec v v0).
+subst; simpl; exists t0 t; auto.
+destruct H; try contradiction; apply IHL; auto.
+Qed.
+
+Lemma NotMem_find_var:
+  forall L v,
+    ~Mem v (map fst_ (map fst_ L)) ->
+    find_var L v = None.
+induction L; intros; simpl in *; auto;
+destruct a; destruct p; rew_map in *; simpl in *;
+case_if.
+elim H; apply Mem_here.
+apply IHL; intro; elim H;
+rewrite Mem_cons_eq; right; auto.
+Qed.
+
+Lemma find_var_Mem:
+forall L v A M,
+  find_var L v = Some (v, A, M) -> Mem (v, A, M) L.
+induction L; intros; [inversion H; subst | ].
+destruct a; destruct p; simpl in *; case_if.
+inversion H; subst; apply Mem_here.
+rewrite Mem_cons_eq; right; apply IHL; auto.
 Qed.
 
 Lemma lc_SL:
-forall L M n,
+forall M L n,
   lc_t_n_LF n M ->
   (forall a b c, Mem (a,b,c) L -> lc_t_LF c) ->
   lc_t_n_LF n (SL L M).
-Admitted.
+induction M; intros; simpl in *;
+try (inversion H; subst; constructor; eapply IHM; eauto).
+destruct v; inversion H; subst.
+constructor; auto.
+destruct (Mem_dec var (map fst_ (map fst_ L)) v). apply eq_var_dec.
+apply Mem_find_var in m; destruct m; destruct H1.
+rewrite H1. replace n with (0+n) by omega.
+apply closed_t_addition; apply H0 with v x. apply find_var_Mem; auto.
+rewrite NotMem_find_var; auto.
+inversion H; subst; constructor; [apply IHM1 | apply IHM2]; auto.
+Qed.
 
-Lemma SL_subst_bte:
-forall L M C k,
-  [C//bte k] (SL L M) = SL L ([C // bte k] M).
-Admitted.
+Lemma SL_bte_subst:
+forall L0 M x k,
+  ~ Mem x (map fst_ (map fst_ L0)) ->
+  (forall v a m, Mem (v, a, m) L0 -> lc_t_LF m) ->
+  [hyp_LF (fte x) // bte k](SL L0 M) =
+  SL L0 [hyp_LF (fte x) // bte k]M.
+induction M; intros; simpl in *;
+try rewrite IHM || (rewrite IHM1; try rewrite IHM2); auto.
+case_if; simpl.
+case_if. rewrite NotMem_find_var; auto.
+destruct v; simpl; repeat case_if; auto.
+destruct (Mem_dec var (map fst_ (map fst_ L0)) v);
+try apply eq_var_dec; [ | rewrite NotMem_find_var]; auto;
+simpl; repeat case_if; auto.
+apply Mem_find_var in m; destruct m as (a, (b, m)); rewrite m; simpl.
+rewrite closed_subst_t_bound_LF with (n:=0); auto; try omega;
+apply H0 with v a; apply find_var_Mem; auto.
+Qed.
+
+Fixpoint FV_L (L: list (var * ty * te_LF)) :=
+match L with
+| nil => \{}
+| (v, A, M) :: L' => used_vars_te_LF M \u FV_L L'
+end.
+
+
+Lemma notin_FV_notin_elem:
+forall x L,
+  x \notin FV_L L ->
+  forall a b c, Mem (a,b,c) L -> x \notin used_vars_te_LF c.
+induction L; intros; simpl in *.
+rewrite Mem_nil_eq in *; contradiction.
+rewrite Mem_cons_eq in H0; destruct H0; [inversion H0; subst | ].
+rewrite notin_union in H; destruct H; auto.
+destruct a; destruct p; rewrite notin_union in H; destruct H;
+apply IHL with (a:=a0) (b:=b); auto.
+Qed.
+
+Lemma SL_extend:
+forall M L0 x A N,
+  x \notin FV_L L0 ->
+  ~Mem x (map fst_ (map fst_ L0)) ->
+  SL ((x, A, N) :: L0) M =
+  [N // fte x](SL L0 M).
+induction M; intros; simpl in *;
+try rewrite IHM || (rewrite IHM1; try rewrite IHM2); auto.
+destruct v; simpl; repeat case_if; auto.
+rewrite NotMem_find_var; auto; simpl; case_if; auto.
+destruct (Mem_dec var (map fst_ (map fst_ L0)) v);
+try apply eq_var_dec; [ | rewrite NotMem_find_var]; auto;
+simpl; repeat case_if; auto.
+apply Mem_find_var in m; destruct m as (a, (b, m)); rewrite m; simpl.
+rewrite closed_subst_t_free_LF; auto.
+apply notin_FV_notin_elem with L0 v a; eauto.
+apply find_var_Mem; eauto.
+Qed.
 
 Theorem main_theorem:
 forall G Gamma M A,
@@ -341,8 +493,9 @@ intros G Gamma M A LC HT; induction HT; intros.
 (* hyp *)
 apply SL_hyp with G Gamma; auto; constructor; auto.
 (* lam *)
-unfold open_LF in *.
-assert (exists x, x \notin L \u used_vars_te_LF (SL L0 M)) by apply Fresh.
+unfold open_LF in *;
+assert (exists x, x \notin L \u used_vars_te_LF (SL L0 M) \u
+       from_list (map fst_ (map fst_ L0)) \u FV_L L0) by apply Fresh;
 destruct H4.
 assert (forall V, Red V A -> lc_t_LF V ->
            Red (SL ((x, A, V) :: L0) [hyp_LF (fte x) // bte 0]M) B).
@@ -355,21 +508,20 @@ apply H2 with a b; auto.
 intros; rewrite Mem_cons_eq in *; destruct H7.
 inversion H7; subst; auto.
 apply H3 with a ; auto.
-rewrite SL_lam. apply reducible_abstraction.
-constructor; apply lc_SL; auto; inversion LC; auto.
-intros; rewrite subst_t_neutral_free_LF with (v:=x); auto.
-rewrite SL_subst_bte.
-(* x is free in all L0 terms, so if it is substituted then it's only in
-[x/0]M itself  - make that into a lemma *)
-replace ([M0 // fte x](SL L0 [hyp_LF (fte x) // bte 0]M)) with
-  (SL ((x, A, M0)::L0) [hyp_LF (fte x) // bte 0]M) by skip.
+simpl in *; intros; apply property_3.
+constructor; auto; constructor; apply lc_SL; auto; inversion LC; auto.
+constructor.
+intros; inversion H6; subst; [ | inversion H12];
+rewrite subst_t_neutral_free_LF with (v:=x); auto.
+replace ([N // fte x]([hyp_LF (fte x) // bte 0](SL L0 M))) with
+  (SL ((x, A, N)::L0) [hyp_LF (fte x) // bte 0]M).
 apply H5; auto.
+rewrite SL_bte_subst; auto; [ | apply notin_Mem; auto].
+rewrite SL_extend; auto; apply notin_Mem; auto.
 (* appl *)
-simpl in *;
-inversion LC; subst; apply IHHT1; auto. apply lc_SL; auto.
+simpl in *; inversion LC; subst; apply IHHT1; auto; apply lc_SL; auto.
 (* box *)
-simpl in *.
-inversion LC; subst; apply property_3.
+simpl in *; inversion LC; subst; apply property_3.
 constructor; constructor; apply lc_SL; auto.
 constructor.
 intros; inversion H2; subst.
@@ -382,200 +534,6 @@ inversion LC; subst; apply IHHT; auto.
 simpl in *;
 inversion LC; subst; apply IHHT; auto;
 rewrite <- H0; apply PPermut_concat_permut; rewrite <- H; PPermut_LF_simpl.
-Qed.
-
-
-(*
-Focus 4.
-inversion LC; subst; rewrite SL_unbox; apply IHHT; auto.
-Focus 4.
-inversion LC; subst; rewrite SL_unbox; apply IHHT; auto;
-rewrite <- H0; apply PPermut_concat_permut; rewrite <- H; PPermut_LF_simpl.
-Focus 3.
-inversion LC; subst; rewrite SL_box; apply property_3.
-constructor; constructor; apply lc_SL; auto.
-constructor.
-intros; inversion H3; subst.
-apply IHHT; auto; rew_concat in *; rewrite <- H; permut_simpl.
-inversion H7.
-Focus 2.
-inversion LC; subst; intros; rewrite SL_lam; apply property_3.
-constructor; auto; constructor; apply lc_SL; auto.
-constructor.
-intros; inversion H5; subst.
-Focus 2. inversion H12.
-assert (exists x, x \notin L \u used_vars_te_LF (SL L0 M)) by apply Fresh.
-destruct H6.
-rewrite subst_t_neutral_free_LF with (v:=x); auto.
-rewrite SL_subst_bte.
-replace ([N // fte x](SL L0 [hyp_LF (fte x) // bte 0]M)) with
-(SL ((x, A, N)::L0) ([hyp_LF (fte x) // bte 0]M)) by (simpl; auto).
-apply H0; auto. skip. rew_map; rewrite <- H1; simpl; rew_concat; auto.
-intros; rewrite Mem_cons_eq in *; destruct H8.
-inversion H8; subst.
-
-Lemma SL'_appl:
-forall M N L,
-  Red (SL' L (appl_LF M N))
-(* hyp *)
-destruct (SL_hyp L G Gamma v A); auto.
-constructor; auto.
-rewrite H3; simpl; case_if; apply H2 with (a:=v).
-apply Mem_PrepSL with (M:=hyp_LF (fte v)); rewrite H3; apply Mem_here.
-(* lam *)
-intros; subst; rewrite SL_lam; apply property_3.
-constructor; auto. constructor. skip.
-constructor.
-intros. inversion H4; subst.
-skip.
-inversion H10.
-(* appl *)
-rewrite SL_appl.
-simpl in *.
-
-
-
-
-
-
-
-
-
-
-
-
-
-
-
-
-
-
-
-
-
-
-
-
-
-
-
-
-
-
-
-
-
-
-
-
-
-
-
-
-
-
-
-
-
-
-
-
-
-
-
-
-
-(*
-(***************************************************)
-Fixpoint SL (L: list (var * ty * te_LF)) (M: te_LF) : te_LF :=
-match L with
-| nil => M
-| (v, A, C) :: L' => [C // fte v](SL L' M)
-end.
-
-
-Lemma nonOcc_SL:
-forall L2 L1 M,
-  (forall v,
-     v \in used_vars_te_LF M -> ~ Mem v (map fst_ (map fst_ L2))) ->
-  SL L1 (SL L2 M) = SL L1 M.
-induction L2; intros; simpl in *; auto.
-destruct a; destruct p.
-rew_map in *; simpl in *.
-replace (SL L1 [ t// fte v] (SL L2 M)) with
-  (SL (L1 & (v, tvar, t)) (SL L2 M)).
-rewrite IHL2.
-rewrite SL_L_app; simpl.
-rewrite closed_subst_t_free_LF; auto.
-intro; specialize H with v; apply H in H0; elim H0; apply Mem_here.
-intros; intro; elim H with (v0:=v0); auto; rew_map in *; simpl in *;
-rewrite Mem_cons_eq; right; auto.
-rewrite <- SL_L_app.
-replace ([t // fte v](SL L2 M)) with (SL ((v, tvar, t)::L2) M)
-                                      by (simpl; auto).
-symmetry; rewrite <- SL_L_app.
-rew_app; auto.
-Qed.
-
-Fixpoint Lc_t_L (L: list (var * ty * te_LF)) :=
-match L with
-| nil => True
-| (v, A, C) :: L' => lc_t_LF C /\ Lc_t_L L'
-end.
-
-Lemma SL_subst_bte:
-forall L M v k,
-  Lc_t_L L ->
-  (forall v' C A, Mem (v', A, C) L -> v' <> v) ->
-  [hyp_LF (fte v) // bte k] (SL L M) = SL L ([hyp_LF (fte v) // bte k] M).
-induction L; intros; simpl in *; auto;
-destruct a; destruct p; destruct H;
-rewrite <- subst_t_comm_LF.
-rewrite IHL; auto.
-intros; apply H0 with (C:=C) (A:=A); rewrite Mem_cons_eq; right; auto.
-auto.
-apply H0 with (C:=t) (A:=t0); apply Mem_here.
-Qed.
-
-(* All the terms are reducible *)
-Fixpoint RedL (L: list (var * ty * te_LF)) : Prop :=
-match L with
-| nil => True
-| (v, A, C) :: L' => Red C A /\ RedL L'
-end.
-
-(* Capture AT LEAS variables from M -- and with good types *)
-Definition GoodL (L: list (var * ty * te_LF)) (M: te_LF) (G: bg_LF) :=
-  forall v,
-    v \in used_vars_te_LF M ->
-    forall A,
-      Mem (v, A) (concat G) ->
-    Mem (v, A) (map fst_ L).
-
-(* Capture ONLY variables from M *)
-Definition NotBadL (L:list (var*ty*te_LF)) (M: te_LF) :=
-  forall v A N,
-    Mem (v, A, N) L ->
-    v \in used_vars_te_LF M.
-
-(* Variable repetition -- not going to happen *)
-Inductive OkL: list (var * ty * te_LF) -> Prop :=
-| OkLNil: OkL (@nil (var * ty * te_LF))
-| OkLCons:
-    forall L v A C, OkL L ->
-                    ~ Mem v (map fst_ (map fst_ L)) ->
-                    OkL ((v, A, C) :: L)
-.
-
-Lemma Mem_map_map:
-forall L (v:var) (A: ty),
-  Mem (v, A) L ->
-  Mem v (map fst_ L).
-induction L; intros; simpl in *.
-rewrite Mem_nil_eq in H; contradiction.
-destruct a; rew_map; rewrite Mem_cons_eq in H; destruct H.
-inversion H; subst; simpl; apply Mem_here.
-simpl; rewrite Mem_cons_eq; right; eauto.
 Qed.
 
 Lemma lc_t_n_LF_subst_t:
@@ -600,821 +558,17 @@ specialize H0 with x; apply H0 in H1;
 apply lc_t_n_LF_subst_t in H0; auto; constructor.
 Qed.
 
-Lemma RedL_split:
-forall L1 L2,
-  RedL (L1++L2) <-> RedL L1 /\ RedL L2.
-induction L1; split; intros; simpl in *; rew_app in *;
-[ split; auto | destruct H; auto | |];
-destruct a; destruct p; destruct H.
-assert (RedL L1 /\ RedL L2) by (eapply IHL1; eauto).
-destruct H1; repeat split; auto.
-destruct H; split; auto; eapply IHL1; split; auto.
-Qed.
-
-Lemma Mem_fst_exists:
-forall (L: list (var * ty * te_LF)) v A,
-  Mem (v, A) (map fst_ L) ->
-  exists N, Mem (v, A, N) L.
-induction L;
-intros; rew_map in *; [rewrite Mem_nil_eq in *; contradiction | destruct a];
-simpl in *; destruct p; rewrite Mem_cons_eq in H; destruct H;
-[inversion H; subst; exists t; apply Mem_here | apply IHL in H; destruct H];
-exists x; rewrite Mem_cons_eq; right; auto.
-Qed.
-
-Lemma Red_SL_hyp:
-forall L v A,
-  RedL L ->
-  OkL L ->
-  NotBadL L (hyp_LF (fte v)) ->
-  Mem (v, A) (map fst_ L) ->
-  Red (SL L (hyp_LF (fte v))) A.
-induction L; intros; simpl in *; unfold NotBadL in *; rew_map in *.
-rewrite Mem_nil_eq in H2; contradiction.
-destruct a; destruct p; simpl in *; destruct H.
-inversion H0; subst.
-destruct L.
-rew_map in *; simpl; rewrite Mem_cons_eq in H2; destruct H2;
-[inversion H2; subst | rewrite Mem_nil_eq in H2; contradiction];
-case_if; auto.
-(* this should lead to contradiction - L should be empty *)
-destruct p; destruct p.
-assert (v0 = v).
-  specialize H1 with (v2:=v0)(A:=t0)(N:=t).
-  rewrite <- in_singleton; apply H1; apply Mem_here.
-assert (v1 = v).
-  specialize H1 with (v2:=v1)(A:=t2)(N:=t1).
-  rewrite <- in_singleton; apply H1; rewrite Mem_cons_eq; right; apply Mem_here.
-subst; rew_map in *; simpl in *.
-elim H9; apply Mem_here.
-Qed.
-
-Lemma SL_lc_t_LF:
-forall L M,
-  Lc_t_L L ->
-  lc_t_LF M ->
-  lc_t_LF (SL L M).
-induction L; intros; simpl in *; auto;
-destruct a; destruct p; destruct H;
-apply lc_t_subst_t_LF_free; eauto; eapply IHL; eauto.
-Qed.
-
-Lemma Var_free_from_List:
-forall L0 (v:var),
-  ~Mem v (map fst_ (map fst_ L0)) ->
-  (forall v' (C: te_LF) (A0: ty), Mem (v', A0, C) L0 -> v' <> v).
-induction L0; intros; simpl.
-rewrite Mem_nil_eq in H0; contradiction.
-destruct a; destruct p; rewrite Mem_cons_eq in H0; destruct H0.
-rew_map in *; simpl in *; inversion H0; subst.
-rewrite Mem_cons_eq in H; intro; destruct H; left; subst; auto.
-eapply IHL0; eauto; intro; rew_map in *; simpl in *; elim H;
-rewrite Mem_cons_eq; right; auto.
-Qed.
-
-Lemma used_vars_te_LF_open_hyp:
-forall M v0 v k,
-  v0 <> v ->
-  v0 \in used_vars_te_LF [hyp_LF (fte v) // bte k] M ->
-  v0 \in used_vars_te_LF M.
-induction M; intros; simpl in *; repeat case_if; simpl in *.
-elim H; subst; rewrite in_singleton in H0; subst; auto.
-destruct v; simpl in *; auto.
-eapply IHM with (v:=v) (k:=S k); auto.
-rewrite in_union in *; destruct H0;
-[left; eapply IHM1 | right; eapply IHM2]; eauto.
-eapply IHM; eauto.
-eapply IHM; eauto.
-Qed.
-
-Lemma SN_subst:
-forall M C v,
-  SN M ->
-  SN C ->
-  SN ([C//fte v]M).
-intros; generalize dependent C; generalize dependent v.
-induction H; intros.
-Lemma subst_value:
-forall M C v,
-  value_LF M -> value_LF [C//v]M.
-induction M; intros; simpl in *; inversion H; subst; auto; constructor.
-Qed.
-simpl; constructor; apply subst_value; auto.
-apply step_SN; intros.
-
-Lemma step_subst:
-forall M C C' v N,
-  lc_t_LF M ->
-  [C//fte v]M |-> [C//fte v]N \/
-  [C//fte v]M |-> [C'//fte v]M.
-induction M; intros; simpl in *; repeat case_if.
-
-
-Lemma subst_red_red_subst:
-forall A B M C v,
-  lc_t_LF C ->
-  Red M A ->
-  Red C B ->
-  Red ([C//fte v]M) A.
-induction A; simpl; intros.
-apply property_1 in H1; auto.
-
-
-Theorem SL_types_reducible:
-forall M G Gamma A,
-  G |= Gamma |- M ::: A ->
-  forall L,
-    OkL L -> RedL L -> GoodL L M (Gamma::G) -> NotBadL L M ->
-    Lc_t_L L -> Red (SL L M) A.
-intros M G Gamma A H; induction H; intros; unfold GoodL in *.
-(* hyp *)
-apply Red_SL_hyp; auto. apply H2; simpl; auto;
-[rewrite in_singleton | rew_concat ];
-auto; rewrite Mem_app_or_eq; left; auto.
-(* lam *)
-assert (exists v, v \notin L \u from_list (map fst_ (concat (Gamma::G))) \u
-                    used_vars_te_LF M \u
-                    used_vars_te_LF (SL L0 M) \u
-       from_list (map fst_ (map fst_ L0)))
-  as HF by apply Fresh; destruct HF as (v);
-rewrite SL_lam; apply reducible_abstraction.
-rewrite <- SL_lam; apply SL_lc_t_LF; auto;
-specialize H with v; apply types_LF_lc_t_LF in H; eauto;
-unfold open_LF in *; constructor;
-apply lc_t_n_LF_subst_t in H; auto; constructor.
-intros.
-Import Arith.
-Fixpoint contains_bte_k (M: te_LF)(k: nat): Prop :=
-match M with
-| hyp_LF (bte n) => if (eq_nat_dec n k) then True else False
-| hyp_LF (fte v) => False
-| lam_LF A M' => contains_bte_k M' (S k)
-| appl_LF M' N' => contains_bte_k M' k \/ contains_bte_k N' k
-| box_LF M' => contains_bte_k M' k
-| unbox_LF M' => contains_bte_k M' k
-end.
-Lemma contains_bte_dec:
-forall M k,
-  { contains_bte_k M k} + {~ contains_bte_k M k}.
-induction M; intros.
-induction v; simpl; [destruct (eq_nat_dec n k); auto | right; tauto].
-specialize IHM with (S k); destruct IHM; simpl; auto.
-specialize IHM1 with k; specialize IHM2 with k; simpl in *;
-destruct IHM1; destruct IHM2; auto; try tauto.
-specialize IHM with k; destruct IHM; simpl; auto.
-specialize IHM with k; destruct IHM; simpl; auto.
-Qed.
-simpl.
-destruct (contains_bte_dec M 0).
-rewrite subst_t_neutral_free_LF with (v:=v); auto.
-rewrite SL_subst_bte; auto.
-Focus 2.
-eapply Var_free_from_List; apply notin_Mem; eauto.
-replace ([M0 // fte v](SL L0 [hyp_LF (fte v) // bte 0]M))
-  with (SL ((v, A, M0) :: L0) [hyp_LF (fte v) // bte 0]M)
-  by (simpl; auto); unfold open_LF in *.
-apply H0; simpl; try split; eauto.
-constructor; eauto; apply notin_Mem; eauto.
-intros; rew_map in *; rew_concat in *; simpl.
-destruct (eq_var_dec v0 v).
-subst; rewrite Mem_cons_eq in *; destruct H11.
-left; auto.
-repeat rewrite notin_union in H6; destruct H6; destruct H12;
-destruct H13; destruct H14.
-apply notin_Mem in H12.
-Lemma Mem_map_fst:
-forall A B L (v:A) (w:B),
-  Mem (v, w) L ->
-  Mem v (map fst_ L).
-induction L; intros; simpl in *.
-rewrite Mem_nil_eq in H; contradiction.
-destruct a; rew_map; simpl; rewrite Mem_cons_eq in *;
-destruct H; [inversion H; subst |]; [left | right]; auto.
-eapply IHL; eauto.
-Qed.
-simpl.
-apply Mem_map_fst in H11; elim H12; auto.
-subst; rewrite Mem_cons_eq in *; destruct H11.
-inversion H11; subst; elim n; auto.
-right; apply H3; simpl; auto.
-apply used_vars_te_LF_open_hyp in H10; auto.
-unfold NotBadL in *; intros.
-rewrite  Mem_cons_eq in *; destruct H10.
-inversion H10; subst.
-Lemma opening_used_vars_contains:
-forall M v k,
-  contains_bte_k M k ->
-  v \in used_vars_te_LF [hyp_LF (fte v) // bte k] M.
-induction M; intros; simpl in *; repeat case_if; simpl; eauto.
-rewrite in_singleton; auto.
-destruct v; simpl in *; repeat case_if; try contradiction.
-destruct H; rewrite in_union; [left| right]; eauto.
-Qed.
-apply opening_used_vars_contains; auto.
-simpl in *.
-Lemma used_vars_subst:
-forall M N k v,
-  v \in used_vars_te_LF M ->
-  v \in used_vars_te_LF [N // bte k] M.
-induction M; intros; simpl in *; repeat case_if; auto.
-rewrite in_empty in H; contradiction.
-rewrite in_union in *; destruct H; [left|right];auto.
-Qed.
-apply used_vars_subst; eapply H4; eauto.
-(* when M does not contain bte 0 *)
-assert (lc_t_LF (SL L0 M)).
-apply SL_lc_t_LF; auto.
-Lemma lc_t_contains_bte:
-forall M k,
-  lc_t_n_LF (S k) M ->
-  ~ contains_bte_k M k ->
-  lc_t_n_LF k M.
-induction M; intros; simpl in *; repeat case_if; try destruct v;
-constructor.
-case_if; [elim H0 | ]; auto. inversion H; subst; omega.
-inversion H; apply IHM; auto.
-inversion H; apply IHM1; auto.
-inversion H; apply IHM2; auto.
-inversion H; apply IHM; auto.
-inversion H; apply IHM; auto.
-Qed.
-apply lc_t_contains_bte; auto.
-assert (lc_t_LF (lam_LF A M)).
-  apply types_LF_lc_t_LF with (G:=G) (Gamma:=Gamma)(A:=A ---> B).
-  eapply t_lam_LF; eauto.
-inversion H10; subst; auto.
-rewrite closed_subst_t_bound_LF with (n:=0); auto.
-unfold open_LF in *.
-clear dependent M0.
-assert (exists x, x \notin L \u used_vars_te_LF M) by apply Fresh; destruct H7.
-rewrite <- closed_subst_t_bound_LF with (v0:=0)(N:=M)(M:=hyp_LF (fte x))(n:=0);
-auto.
-Focus 2.
-apply lc_t_contains_bte; auto.
-assert (lc_t_LF (lam_LF A M)).
-  apply types_LF_lc_t_LF with (G:=G) (Gamma:=Gamma)(A:=A ---> B).
-  eapply t_lam_LF; eauto.
-inversion H8; subst; auto.
-assert (lc_t_LF M).
-apply lc_t_contains_bte; auto.
-assert (lc_t_LF (lam_LF A M)).
-  apply types_LF_lc_t_LF with (G:=G) (Gamma:=Gamma)(A:=A ---> B).
-  eapply t_lam_LF; eauto.
-inversion H8; subst; auto.
-apply H0; auto.
-rewrite closed_subst_t_bound_LF with (n:=0); auto; intros.
-apply H3; simpl; auto.
-rew_concat in H11; rewrite Mem_cons_eq in H11; destruct H11; auto;
-inversion H11; subst; rewrite notin_union in H7; destruct H7; contradiction.
-unfold NotBadL in *; intros.
-rewrite closed_subst_t_bound_LF with (n:=0); auto; intros. simpl in *;
-eapply H4; eauto.
-(* appl *)
-unfold NotBadL in *; simpl in *.
-Lemma NotBadL_appl_split1:
-forall L M N
-   (NotBad: ∀ (v : var) (A : ty) (N0 : te_LF),
-       Mem (v, A, N0) L → v \in used_vars_te_LF M \u used_vars_te_LF N),
-  exists L1,
-    (forall e, Mem e L1 -> Mem e L) /\
-    NotBadL L1 M.
-induction L; intros.
-exists (@nil (var * ty * te_LF)); split.
-auto.
-unfold NotBadL; intros; rewrite Mem_nil_eq in H; contradiction.
-destruct (IHL M N).
-intros; apply NotBad with A N0; rewrite Mem_cons_eq; right; auto.
-destruct H; destruct a; destruct p;
-specialize NotBad with v t0 t; rewrite in_union in NotBad.
-destruct NotBad; [apply Mem_here | exists ((v,t0,t)::x) | exists x];
-split; auto.
-intros. rewrite Mem_cons_eq in *; destruct H2; [left | right]; auto.
-unfold NotBadL in *; intros; rewrite Mem_cons_eq in *; destruct H2;
-[inversion H2; subst | apply H0 in H2]; auto.
-intros; rewrite Mem_cons_eq; right; auto.
-Qed.
-simpl.
-apply NotBadL_appl_split1 in H4; destruct H4 as (L1, (H4, H6)).
-rewrite SL_appl; simpl in *.
-apply IHtypes_LF1 with (G:=G)(Gamma:=Gamma); auto.
-intros; apply H3; simpl; auto; rewrite in_union; left; auto.
-unfold NotBadL in *; intros; simpl in *.
-apply H6 with A0 N0.
-apply H4 in H7.
-
-(*
-(* This assumes that bte 0 actually was present in M
- -- we need to add a case where it was not! *)
-skip.
-(* appl *)
-
-(******************************************************************)
-
-
-
-(* These two lemmas may be a little technical because of the way subsets are
-   implemented *)
-(* fset_finite? *)
-Lemma types_LF_term_vars_in_all_vars:
-forall M G Gamma A,
-  G |= Gamma |- M ::: A ->
-  used_vars_te_LF M \c from_list (flat_map (fun x => map fst_ x) (Gamma::G)).
-Admitted.
-
-Lemma types_empty_LF_no_free_vars:
-forall M G A,
-  emptyEquiv_LF G |= nil |- M ::: A ->
-  used_vars_te_LF M = \{}.
-Admitted.
-
-
-Lemma apply lc_t_contains_bte; auto.
-apply lc_t_contains_bte; auto.
-types_LF_lc_t_LF:
-forall G Gamma M A,
-  G |= Gamma |- M ::: A -> lc_t_LF M.
-intros; induction H; constructor; try apply IHHT;
-unfold open_LF in *; auto.
-assert (exists x, x \notin L) by apply Fresh; destruct H1;
-assert (x \notin L) by auto;
-specialize H0 with x; apply H0 in H1;
-apply lc_t_n_LF_subst_t in H0; auto; constructor.
-Qed.
-
-Fixpoint S (L: list (var * te_LF * ty)) (M: te_LF) : te_LF :=
-match L with
-| nil => M
-| (v, C, A) :: L' => [C // fte v] (S L' M)
-end.
-
-
-Inductive GoodS: list (var * te_LF * ty) -> te_LF -> Prop :=
-| nilS: forall M, GoodS nil M
-| consS:
-    forall L M v C A,
-      GoodS L M ->
-      v \in used_vars_te_LF (S L M) ->
-      lc_t_LF C ->
-      Red C A ->
-      GoodS ((v, C, A)::L) M
-.
-
-Definition fullS L M := GoodS L M /\ used_vars_te_LF (S L M) = \{}.
-
-Lemma S_lam:
-forall L A M,
-  S L (lam_LF A M) = lam_LF A (S L M).
-induction L; intros; simpl in *; eauto;
-destruct a; destruct p; rewrite IHL; eauto.
-Qed.
-
-Lemma S_appl:
-forall L M N,
-  S L (appl_LF M N) =
-  appl_LF (S L M) (S L N).
-induction L; intros; simpl in *; eauto;
-destruct a; destruct p; rewrite IHL; eauto.
-Qed.
-
-Lemma S_box:
-forall L M,
-  S L (box_LF M) = box_LF (S L M).
-induction L; intros; simpl in *; eauto;
-destruct a; destruct p; rewrite IHL; eauto.
-Qed.
-
-Lemma S_unbox:
-forall L M,
-  S L (unbox_LF M) = unbox_LF (S L M).
-induction L; intros; simpl in *; eauto;
-destruct a; destruct p; rewrite IHL; eauto.
-Qed.
-
-Lemma S_hyp:
-forall L v A,
-  fullS L (hyp_LF (fte v)) ->
-  Red (S L (hyp_LF (fte v))) A.
-unfold fullS; intros; destruct H.
-generalize dependent A;
-generalize dependent v;
-induction L; intros; simpl in *.
-assert (v \in \{v}) by (rewrite in_singleton; auto);
-rewrite H0 in H1; apply notin_empty in H1; contradiction.
-destruct a; destruct p; simpl in *.
-inversion H; subst.
-Admitted. (* !!! *)
-
-Lemma GoodS_lc_t:
-forall L M,
-  GoodS L M ->
-  forall C,
-    Mem C (map snd_ (map fst_ L)) -> lc_t_LF C.
-induction L; intros; simpl in *; rew_map in *.
-rewrite Mem_nil_eq in H0; contradiction.
-destruct a; destruct p; simpl in *; rewrite Mem_cons_eq in H0;
-inversion H; subst; destruct H0; subst; eauto.
-Qed.
-
-Lemma subst_t_bound_subst_free_vars:
-forall L M v k,
-  GoodS L M ->
-  ~ Mem v (map fst_ (map fst_ L)) ->
-  [hyp_LF (fte v) // bte k](S L M) =
-  S L ([hyp_LF (fte v) // bte k] M).
-induction L; intros; simpl in *; auto.
-destruct a; destruct p; rew_map in *;
-assert ( v0 <> v) by (intro; elim H0; rewrite Mem_cons_eq; left; auto);
-simpl in *; rewrite <- subst_t_comm_LF; auto.
-inversion H; subst; rewrite IHL; auto.
-intro; elim H0; rewrite Mem_cons_eq; right; auto.
-apply GoodS_lc_t with (C:=t0) in H; auto; rew_map; simpl; apply Mem_here.
-Qed.
-
-Lemma S_lc_t_LF:
-forall L M,
-  GoodS L M ->
-  lc_t_LF M ->
-  lc_t_LF (S L M).
-induction L; intros; simpl in *; eauto;
-destruct a; destruct p.
-apply lc_t_subst_t_LF_free; [ | eapply IHL; eauto];
-inversion H; subst; auto.
-Qed.
-
-Lemma GoodS_lam:
-forall L0 L M A,
-  GoodS L (lam_LF A M) ->
-  forall v, v \notin L0 ->
-    GoodS L ([hyp_LF (fte v)//bte 0]M).
-induction L; intros; simpl in *; try constructor;
-destruct a; destruct p; constructor; inversion H; subst; auto.
-eapply IHL; eauto.
-skip. (* !!! *)
-Qed.
-
-Lemma main_attempt1:
-forall G Gamma M A L,
-  G |= Gamma |- M ::: A ->
-  fullS L M ->
-  Red (S L M) A.
-unfold fullS in *;
-intros; assert (lc_t_LF M) by (eapply types_LF_lc_t_LF in H; eauto);
-generalize dependent L. induction H; intros; subst.
-(* hyp *)
-apply S_hyp; unfold fullS; auto.
-(* lam *)
-destruct H2; rewrite S_lam; apply reducible_abstraction; auto; intros.
-rewrite <- S_lam; apply S_lc_t_LF; auto.
-unfold open_LF in *;
-assert (exists v, v \notin L \u used_vars_te_LF (S L0 M) \u
-       from_list (map fst_ (map fst_ L0))) as HF
-  by apply Fresh; destruct HF;
-rewrite subst_t_neutral_free_LF with (v:=x); eauto;
-rewrite subst_t_bound_subst_free_vars.
-assert (x \in used_vars_te_LF (S L0 [hyp_LF (fte x) // bte 0]M) \/
-        x \notin used_vars_te_LF (S L0 [hyp_LF (fte x) // bte 0]M)).
-  skip. (* !!! *)
-destruct H7.
-(* in *)
-replace ([M0 // fte x](S L0 [hyp_LF (fte x) // bte 0]M))
-  with (S ((x, M0, A) :: L0) [hyp_LF (fte x) // bte 0] M) by (simpl; auto).
-apply H0; eauto.
-inversion H1; subst; apply lc_t_subst_t_LF_bound; auto; constructor.
-simpl. split.
-constructor; auto; apply GoodS_lam with (L0:=L)(A:=A); eauto.
-rewrite <- subst_t_bound_subst_free_vars.
-rewrite <- subst_t_neutral_free_LF.
-Admitted.
-
-Lemma main_conclusion1:
+Theorem SN_Lang:
 forall G M A,
   emptyEquiv_LF G |= nil |- M ::: A ->
   SN M.
-intros; apply property_1 with (A:=A).
+intros; apply property_1 with A.
 apply types_LF_lc_t_LF in H; auto.
-apply main_attempt1 with (L:=nil) in H; auto.
-split; simpl in *; [constructor | apply types_empty_LF_no_free_vars in H; auto].
-Qed.
-
-
-(* Idea: gather all free variables from a term,
-         substitute them with reducible terms of appropriate type
-         conclude that the resulting term is reducible *)
-
-Fixpoint subst_free_vars (D: list (var*ty))
-         (L: list te_LF) N :=
-match D, L with
-| nil, _ => N
-| _, nil => N
-| (v, _ )::V', l::L' => [l // fte v] (subst_free_vars V' L' N)
-end.
-
-Fixpoint subst_typing G (L: list te_LF) (D: list (var * ty)) :=
-match L, D with
-| nil, nil => True
-| M ::L', (v, A) :: D' =>
-  emptyEquiv_LF G |= nil |- M ::: A /\ (subst_typing G L' D')
-| _, _ => False
-end.
-
-Fixpoint red_list (L: list te_LF) (D: list (var * ty)) :=
-match L, D with
-| nil, nil => True
-| M :: L', (v, A):: D' => Red M A /\ red_list L' D'
-| _, _ => False
-end.
-
-Lemma subst_free_vars_notin:
-forall D L,
-  red_list L D ->
-  ok_LF D nil ->
-  forall v,
-    ~ Mem v (map fst_ D) ->
-    subst_free_vars D L (hyp_LF (fte v)) = hyp_LF (fte v).
-induction D; intros; simpl in *; auto; destruct a; rew_map in *; simpl in *;
-rewrite Mem_cons_eq in *; destruct L; auto.
-simpl in *; destruct H; inversion H0; subst.
-rewrite IHD; simpl; eauto.
-case_if; auto; inversion H3; subst. elim H1; left; auto.
-inversion H0; subst; eapply ok_LF_used_weakening in H8; auto.
-Qed.
-
-Lemma ok_LF_step:
-forall D v (A:ty) U,
-  ok_LF ((v, A) :: D) U -> ~ Mem v (map fst_ D).
-induction D; intros; rew_map.
-rewrite Mem_nil_eq; auto.
-destruct a; intro nn; rewrite Mem_cons_eq in nn; simpl in *; destruct nn; subst.
-inversion H; inversion H5; subst; elim H10; apply Mem_here.
-specialize IHD with v A (v0::U).
-apply ok_LF_permut with (G':= (v0,t) :: (v, A) :: D) in H; [|permut_simpl].
-inversion H; subst; apply IHD in H6; contradiction.
-Qed.
-
-Lemma used_vars_te_LF_subst_t:
-forall N C k,
-  used_vars_te_LF ([C // bte k] N) = used_vars_te_LF N \/
-  used_vars_te_LF ([C // bte k] N) = used_vars_te_LF C \u used_vars_te_LF N.
-induction N; intros; simpl in *.
-destruct v; case_if; simpl;
-[right; rewrite union_empty_r | left | left ]; auto.
-destruct IHN with C (S k); rewrite <- H; [left | right]; auto.
-destruct IHN1 with C k; destruct IHN2 with C k; rewrite H; rewrite H0;
-[left | right | right | right]; auto.
-rewrite <- union_comm_assoc; auto.
-rewrite union_assoc; auto.
-rewrite <- union_comm_assoc.
-rewrite <- union_assoc.
-assert (forall N,
-          used_vars_te_LF C \u used_vars_te_LF C \u N = used_vars_te_LF C \u N).
-intros; rewrite union_assoc; rewrite union_same; auto.
-rewrite H1; auto.
-destruct IHN with C k; rewrite H; [left | right]; auto.
-destruct IHN with C k; rewrite H; [left | right]; auto.
-Qed.
-
-Lemma Mem_map_fst:
-forall A B D (x:A) (t:B),
-  Mem (x, t) D -> Mem x (map fst_ D).
-induction D; intros.
-rewrite Mem_nil_eq in H; contradiction.
-destruct a; rewrite Mem_cons_eq in H; destruct H; rew_map; simpl.
-inversion H; subst; apply Mem_here.
-rewrite Mem_cons_eq; right; eauto.
-Qed.
-
-
-Lemma free_vars_empty_subst_typing:
-forall G L D,
-  subst_typing G L D ->
-  forall t, Mem t L -> used_vars_te_LF t = \{}.
-induction L; destruct D; intros; simpl in *.
-rewrite Mem_nil_eq in H0; contradiction.
-contradiction.
-contradiction.
-rewrite Mem_cons_eq in H0; destruct H0; subst; destruct p; destruct H.
-eapply types_empty_LF_no_free_vars; eauto.
-eauto.
-Qed.
-
-Lemma subst_free_vars_single_occ:
-forall D L A G t v0 v,
-  subst_typing G (t::L) ((v0,A)::D) ->
-  ok_LF ((v0, A) :: D) nil ->
-  (v = v0 -> [t // fte v0](subst_free_vars D L (hyp_LF (fte v))) = t) /\
-  (v <> v0 ->  [t // fte v0](subst_free_vars D L (hyp_LF (fte v))) =
-    subst_free_vars D L (hyp_LF (fte v))).
-intros.
-remember (t::L) as L'.
-remember ((v0,A)::D) as D'.
-generalize dependent A;
-generalize dependent t;
-generalize dependent v0;
-generalize dependent v;
-generalize dependent D;
-generalize dependent L.
-(*
-induction H.
-generalize dependent G;
-generalize dependent D';
-generalize dependent L'.
-induction L'; destruct D'; intros; simpl in *;
-inversion HeqL'; inversion HeqD'; subst; split; intros;
-destruct H.
-inversion H0; subst; clear HeqL' HeqD' H7 H0.
-destruct IHD' with (t0::L) L D v0 v0 t0 G A; auto.
-skip.
-assert (v0 <> v1) by (intro; subst; elim H9; apply Mem_here).
-destruct IHD with L t1 G t v1 v0; auto. skip.
-destruct H1;
-destruct IHD with L A G t0 v0 v0; auto. skip.
-apply H5 in H3; rewrite H3; apply H11 in H2; rewrite H2; auto.
-destruct H; inversion H0; subst; inversion H8; subst;
-assert (v0 <> v1) by (intro; subst; elim H9; apply Mem_here).
-destruct H2.
-destruct IHD with L t1 G t v1 v; auto. skip.
-destruct (eq_var_dec v v1).
-apply H5 in e; rewrite e; apply closed_subst_t_free_LF.
-erewrite free_vars_empty_subst_typing; eauto.
-destruct IHD with A L t0 v0 v0. skip.
-apply H3 in H0; rewrite H0.
-apply H4 in H1; rewrite H1; auto.
-*)
-Admitted.
-
-Lemma subst_free_vars_hyp:
-forall G L D,
-  ok_LF D nil ->
-  subst_typing G L D ->
-  forall v A,
-    Mem (v, A) D ->
-    exists N,
-      Mem N L /\
-      subst_free_vars D L (hyp_LF (fte v)) = N.
-Admitted.
-
-Lemma red_list_Red:
-forall L D N,
-  red_list L D ->
-  Mem N L ->
-  exists A, Red N A.
-induction L; destruct D; intros; simpl in *.
-rewrite Mem_nil_eq in H0; contradiction.
-contradiction.
-contradiction.
-destruct p; destruct H.
-rewrite Mem_cons_eq in H0; destruct H0; eauto;
-inversion H0; subst; exists t; auto.
-Qed.
-
-Lemma subst_free_vars_hyp_Red:
-forall G D L,
-  red_list L D ->
-  ok_LF D nil ->
-  subst_typing G L D ->
-  forall v A,
-    Mem (v, A) D ->
-    Red (subst_free_vars D L (hyp_LF (fte v))) A.
-intros.
-assert (exists N, Mem N L /\
-        subst_free_vars D L (hyp_LF (fte v)) = N).
-eapply subst_free_vars_hyp; eauto.
-destruct H3 as (N, (H3, H4)).
-rewrite H4.
-Admitted.
-
-(* !!! *)
-Lemma lc_t_subst_free_vars:
-forall L D k M,
-  (forall N, Mem N L -> lc_t_LF N) ->
-  lc_t_n_LF k M ->
-  lc_t_n_LF k (subst_free_vars D L M).
-Admitted.
-
-(* !!! *)
-Lemma subst_t_bound_subst_free_vars:
-forall L D M v k,
-  ~ Mem v (map fst_ D) ->
-  [hyp_LF (fte v) // bte k](subst_free_vars D L M) =
-  subst_free_vars D L ([hyp_LF (fte v) // bte k] M).
-Admitted.
-
-Lemma types_LF_lc_t_LF:
-forall G Gamma M A,
-  G |= Gamma |- M ::: A -> lc_t_LF M.
-intros; induction H; simpl in *; constructor; eauto.
-Admitted.
-
-Lemma subst_free_vars_type:
-forall G Gamma M A L G',
-  G |= Gamma |- M ::: A ->
-  concat (Gamma::G) *=* G' ->
-  subst_typing G L G' ->
-  G |= Gamma |- subst_free_vars G' L M ::: A.
-Admitted.
-
-Lemma map_permut_fst:
-forall (G: list (var * ty)) G',
-  G *=* G' -> map fst_ G *=* map fst_ G'.
-Admitted.
-
-Lemma subst_free_vars_lam:
-forall D L A M,
-  subst_free_vars D L (lam_LF A M) = lam_LF A (subst_free_vars D L M).
-induction D; intros; simpl in *; eauto;
-destruct a; destruct L; auto. rewrite IHD; simpl; auto.
-Qed.
-
-Lemma subst_free_vars_appl:
-forall D L M N,
-  subst_free_vars D L (appl_LF M N) =
-  appl_LF (subst_free_vars D L M) (subst_free_vars D L N).
-induction D; intros; simpl in *; eauto;
-destruct a; destruct L; auto; rewrite IHD; simpl; auto.
-Qed.
-
-Lemma subst_free_vars_box:
-forall D L M,
-  subst_free_vars D L (box_LF M) = box_LF (subst_free_vars D L M).
-induction D; intros; simpl in *; eauto;
-destruct a; destruct L; auto; rewrite IHD; simpl; auto.
-Qed.
-
-Lemma subst_free_vars_unbox:
-forall D L M,
-  subst_free_vars D L (unbox_LF M) = unbox_LF (subst_free_vars D L M).
-induction D; intros; simpl in *; eauto;
-destruct a; destruct L; auto; rewrite IHD; simpl; auto.
-Qed.
-
-Lemma subst_typing_lc:
-forall L G G0 M,
-  subst_typing G0 L G ->
-  Mem M L ->
-  lc_t_LF M.
-induction L; destruct G; simpl; intros.
-rewrite Mem_nil_eq in H0; contradiction.
-contradiction.
-contradiction.
-destruct p; rewrite Mem_cons_eq in *; destruct H0; destruct H.
-inversion H0; subst.
+apply main_theorem with (L:=nil) in H.
+rewrite SL_nil in H; auto.
 apply types_LF_lc_t_LF in H; auto.
-eapply IHL with (G:=G); eauto.
+rew_concat; rew_map; clear H M A.
+induction G; simpl; rew_concat; auto.
+intros; rewrite Mem_nil_eq in *; contradiction.
+intros; rewrite Mem_nil_eq in *; contradiction.
 Qed.
-
-Theorem subst_types_reducible:
-forall M G Gamma A L G'
-  (H_lc: lc_t_LF M)
-  (HT: emptyEquiv_LF G |= nil |- M ::: A)
-  (HPermut: concat (Gamma :: G) *=* G')
-  (HRed: red_list L G')
-  (HRedType: subst_typing G L G'),
-  Red (subst_free_vars G' L M) A.
-intros; generalize dependent L; generalize dependent G';
-induction HT; intros; inversion H_lc; subst; rew_app in *; rew_concat in *;
-simpl in *.
-(* hyp *)
-apply subst_free_vars_hyp_Red with (G:=G); auto.
-apply ok_LF_permut with (G:=concat (Gamma::G)); unfold ok_Bg_LF in Ok; auto.
-apply Mem_permut with (l:=Gamma ++ concat G); auto;
-rewrite Mem_app_or_eq; left; auto.
-(* lam *)
-intros; rewrite subst_free_vars_lam; apply property_3.
-repeat constructor; auto; apply lc_t_subst_free_vars; auto.
-intros; eapply subst_typing_lc; eauto.
-constructor.
-intros; inversion H1; subst; [ | inversion H8].
-assert (exists x, x\notin L \u from_list (map fst_ G')
-       \u used_vars_te_LF (subst_free_vars G' L0 M))
-  by apply Fresh. destruct H2.
-unfold open_LF in *; rewrite subst_t_neutral_free_LF with (v:=x).
-rewrite subst_t_bound_subst_free_vars.
-specialize H0 with x L0 G';
-assert (x \notin L) as HH by eauto.
-apply H0 with ((x, A)::G') (N::L0) in HH; simpl in *;
-auto.
-apply lc_t_subst_t_LF_bound; auto; constructor.
-rew_app; rew_concat; rewrite HPermut; auto.
-apply notin_Mem; rew_concat in H2; eauto.
-eauto.
-(* appl *)
-rewrite subst_free_vars_appl; eapply IHHT1 with (G:=G)(Gamma:=Gamma); eauto.
-apply lc_t_subst_free_vars; auto; intros; eapply subst_typing_lc; eauto.
-eapply subst_free_vars_type; auto.
-(* box *)
-apply property_3.
-constructor; apply lc_t_subst_free_vars; auto;
-intros; eapply subst_typing_lc; eauto.
-constructor.
-intros. inversion H; subst.
-rewrite subst_free_vars_box in H0; inversion H0; subst.
-eapply IHHT; eauto.
-rew_app; rewrite <- HPermut; auto.
-rewrite subst_free_vars_box in H3; inversion H3.
-(* unbox *)
-rewrite subst_free_vars_unbox; eapply IHHT; eauto.
-rewrite subst_free_vars_unbox; apply IHHT; auto.
-rewrite <- HPermut; rew_concat; permut_simpl;
-apply PPermut_concat_permut in H; rewrite <- H; rew_concat; permut_simpl.
-Qed.
-*)
